Util.dfy
@@ -53,6 +53,40 @@ module Util {
       digitString + NatToString(n/10)
   }
 
+  lemma HashTagNotInNatString(n: nat)
+    ensures '#' !in NatToString(n)
+  { }
+
+  lemma NatToStringInjective(n1: nat, n2: nat)
+    requires n1 != n2
+    ensures NatToString(n1) != NatToString(n2)
+  /*
+  {
+    if n1 == 0 {
+      //trivial
+    } else {
+      var digit1 := n1 % 10;
+      var digitString1 := ['0' + digit1 as char];
+
+      var digit2 := n2 % 10;
+      var digitString2 := ['0' + digit2 as char];
+
+      assert |digitString1| == |digitString2|;
+
+      assume NatToString(n1/10) != NatToString(n2/10);
+
+      if digit1 != digit2 {
+        //assert ('0'+ digit1 as char) != ('1'+ digit2 as char);
+        assume false;
+      } else {
+        assume n1/10 != n2/10;
+        NatToStringInjective(n1/10, n2/10);
+
+      }
+    }
+  }
+  */
+
   function method BoolToString(b: bool) : string {
     if b then "true" else "false"
   }
